\begin{answer}

For convenience, let 
\begin{equation}
    L = \KL(P(X,Y)\|Q(X,Y)) = \sum_x \sum_y P(x,y) \log\frac{P(x,y)}{Q(x,y)}
\end{equation}
and 
\begin{equation}
    R = \KL(P(X)\|Q(X)) + \KL(P(Y|X)\|Q(Y|X))
\end{equation}

Then, use the fact that $P(x)P(y|x) = P(x,y)$,
\begin{align*}
R &= \sum_x P(x) \log\frac{P(x)}{Q(x)} + \sum_x P(x) \left(\sum_y P(y|x) \log\frac{P(y|x)}{Q(y|x)}\right) \\
&= \sum_x P(x) \log\frac{P(x)}{Q(x)} + \sum_x \sum_y P(x)P(y|x) \log\frac{P(y|x)}{Q(y|x)} \\
&= \sum_x P(x) \log\frac{P(x)}{Q(x)} + \sum_x \sum_y P(x,y) \log\frac{P(y|x)}{Q(y|x)} \\
&= \sum_x \sum_y P(x,y) \log\frac{P(x)}{Q(x)} + \sum_x \sum_y P(x,y) \log\frac{P(y|x)}{Q(y|x)} \\
&= \sum_x \sum_y P(x,y) \left(\log\frac{P(x)}{Q(x)} + \log\frac{P(y|x)}{Q(y|x)}\right) \\
&= \sum_x \sum_y P(x,y) \log\frac{P(x)P(y|x)}{Q(x)Q(y|x)} \\
&= \sum_x \sum_y P(x,y) \log\frac{P(x,y)}{Q(x,y)} \\
&= L
\end{align*}


\end{answer}
