\begin{answer}

Given
\begin{equation}
    \alpha_{i, (t+1)}
 			= \frac{\alpha_{i, t} \exp(-\hat{w}_t f_t(x_i) y_i)}{Z_t},
\end{equation}
From induction,
\begin{equation}
    \alpha_{i, (t+1)}
 			= \frac{\exp(-\hat{w}_t f_t(x_i) y_i)}{Z_t} \cdot \frac{\exp(-\hat{w}_{t-1} f_{t-1}(x_i) y_i)}{Z_{t-1}} \cdots \alpha_{i, 1}
\end{equation}

Given $\alpha_{i, 1}$ is $\frac{1}{n}$, the above equation can be written as 

\begin{equation}
    \alpha_{i, (t+1)} = \frac{1}{n} \prod_{t=1}^T \frac{\exp(-\hat{w}_t f_t(x_i) y_i)}{Z_t}
\end{equation}

equivalently, 
\begin{equation}
    \prod_{t=1}^T Z_t \cdot \alpha_{i, (t+1)} \cdot n= \prod_{t=1}^T \exp(-\hat{w}_t f_t(x_i) y_i)
\end{equation}

Given the definition of $f(x)$, we have the following 
\begin{equation}
    \exp(-f(x_i)y_i) = \exp\left(-\sum_{t=1}^{T} \hat{w}_t f_t(x_i)y_i\right) = \prod_{t=1}^{T} \exp\left(-\hat{w}_t f_t(x_i)y_i\right)
\end{equation}


Combine (19) and (20), 
\begin{equation}
    \exp(-f(x_i)y_i) = \prod_{t=1}^T Z_t \cdot \alpha_{i, (t+1)} \cdot n
\end{equation}

Sum all $n$ observations, 
\begin{equation}
    \sum_{i=1}^{n} \exp(-f(x_i)y_i) = \sum_{i=1}^{n} \alpha_{i, (t+1)} \cdot \prod_{t=1}^T Z_t \cdot n
\end{equation}

$\alpha_{i, (t+1)}$ is a normalized parameter, so 
\begin{equation}
    \sum_{i=1}^{n} \alpha_{i, (t+1)} = 1
\end{equation}

Replacing (23) into (22), we get
\begin{equation}
    \frac{1}{n} \sum_{i=1}^n \exp(-f(x_i)y_i)= \prod_{t=1}^T Z_t
\end{equation}
\end{answer}