\begin{answer}

Given exponential family distribution as follows
\begin{equation*}
p(y ; \eta) = b(y)\exp(\eta y - a(\eta)).
\end{equation*}

Apply the hint
\begin{equation*}
\int \frac{\partial}{\partial \eta} p(y; \eta)dy = \frac{\partial}{\partial \eta} \int p(y; \eta)dy = \frac{\partial}{\partial \eta} 1 = 0
\end{equation*}

then 

\begin{equation*}
\frac{\partial}{\partial \eta} p(y; \eta) 
= b(y) \frac{\partial}{\partial \eta} \left( \exp(\eta y - a(\eta)) \right) = b(y) \exp(\eta y - a(\eta)) \left( y - \frac{\partial a(\eta)}{\partial \eta} \right) = p(y; \eta) \left( y - \frac{\partial a(\eta)}{\partial \eta} \right) 
\end{equation*}
        

Substituting $\frac{\partial}{\partial \eta} p(y; \eta)$ back into the integral, we get:

\begin{equation*}
\int p(y; \eta) \left( y - \frac{\partial a(\eta)}{\partial \eta} \right) dy = 0.
\end{equation*}

which is equivalent to 
\begin{equation*}
    \int p(y; \eta)ydy = \frac{\partial a(\eta)}{\partial \eta} \int p(y; \eta)dy = \frac{\partial a(\eta)}{\partial \eta}
\end{equation*}

The left hand side of the above equation is the definition of $\mathbb{E}[Y; \eta]$

\end{answer}
