\begin{answer} 

(i) prove equation(9) is sufficient to equation(8)

Replacing $\beta=X^\top (XX^\top)^{-1}\vec{y}+\zeta $ in  $J(\beta)=\frac{1}{2n}\|X\beta-\vec{y}\|_2^2.$,

\begin{equation}
    \frac{1}{2n}\|X\beta-\vec{y}\|_2^2 =  \frac{1}{2n}\|X\left(X^\top (XX^\top)^{-1}\vec{y}+\zeta\right)-\vec{y}\|_2^2 = \frac{1}{2n}\|\vec{y}+X\zeta-\vec{y}\|_2^2
\end{equation}

Given $\zeta$ in orthogonal to all the data $x^{(i)}$, the above equation equals 0

(ii) prove equation(9) is necessary to equation(8)

Given $J(\beta) = 0$, we get 
\begin{equation}
    X\beta-\vec{y} = 0,  X\beta = \vec{y}
\end{equation}

Let $\rho = X^\top(X X\top)^{-1}\vec{y}$, then 
\begin{equation}
    X\rho = X X^\top(X X^\top)^{-1}\vec{y} = \vec{y}
\end{equation}

Let equation (11) - equation (12), we get
\begin{equation}
    X(\beta - \rho) = 0
\end{equation}
AKA 
\begin{equation}
    \beta = \rho + \zeta = X^\top(X X\top)^{-1}\vec{y} + \zeta
\end{equation}

Above all, (9) is both sufficient and necessary to (8)

\end{answer}
