\begin{answer}

The variance of a sum of random variables is given by the following
\begin{equation}
    \text{Var}\left(\sum_{i=1}^{B} T_i(x)\right) = \sum_{i=1}^{B} \text{Var}(T_i(x)) + 2\sum_{i<j} \text{Cov}(T_i(x), T_j(x))
\end{equation}

where
\begin{equation}
    \text{Var}(T_i(x)) = \sigma^2\ \text{for i = 1, \cots, B}
\end{equation}

and 
\begin{equation}
    \text{Cov}(T_i(x), T_j(x)) =  Corr(X,Y) \sqrt{Var(X)}\sqrt{Var(Y)} = \rho\sigma^2
\end{equation}

Replacing (15), (16) in (14)
\begin{equation}
\text{Var}\left(\sum_{i=1}^{B} T_i(x)\right) = B\sigma^2 + 2\sum_{i<j} \rho\sigma^2 = B\sigma^2 + B(B-1)\rho\sigma^2
\end{equation}

Given (17), the variance of the average is given by 
\begin{equation}
\text{Var}\left(\frac{1}{B}\sum_{i=1}^{B}T_i(x)\right) = \frac{1}{B^2}\left[B\sigma^2 + B(B-1)\rho\sigma^2\right] = \frac{\sigma^2}{B} + \frac{(B-1)\rho\sigma^2}{B}
\end{equation}

(18) can be simplified as 
\begin{equation}
\text{Var}\left(\frac{1}{B}\sum_{i=1}^{B}T_i(x)\right) = \rho\sigma^2 + \frac{1-\rho}{B}\sigma^2
\end{equation}

\end{answer}