\begin{answer}

Expand the equation of MSE
\begin{equation}
\text{MSE}(h) = \E[(Y - h(X))^2] = \E = \E[(Y - T(X))^2] + \E[(T(X) - h(X))^2] + 2\E[(Y - T(X))(T(X) - h(X))]
\end{equation}

where 
\begin{equation}
    \text{CE}(h) = \E[(T(X) - h(X))^2]
\end{equation}

From the definition of $T(x) = \Pr [Y =1 \mid h(X) = h(x)]$, we have 
\begin{equation}
    T(X) = \E[Y | h(X)]
\end{equation} 

Apply the law of total variance, 

\begin{equation}
\text{Var}[Y] = \E[\text{Var}[Y | h(X)]] + \text{Var}[\E[Y | h(X)]] = \E[\text{Var}[Y | h(X)]] + \text{Var}[T(X)]
\end{equation} 

Given the definition of conditional variance 
\begin{equation}
    \text{Var}[Y | h(X)] = \E\left[(Y - T(X))^2 \mid h(X)\right]
\end{equation}
we get 
\begin{equation}
    \E[\text{Var}[Y | h(X)]] = \E[(Y - T(X))^2]
\end{equation}
so we can rewrite $\text{Var}[Y]$ as:

\begin{equation}
    \text{Var}[Y] = \E[(Y - T(X))^2] + \text{Var}[T(X)]
\end{equation}


For the cross-term \(2\E[(Y - T(X))(T(X) - h(X))]\), we note that \(T(X) = \E[Y | h(X)]\), so \(\E[Y - T(X) | h(X)] = 0\). This implies that the cross-term is zero:

\begin{equation}
2\E[(Y - T(X))(T(X) - h(X))] = 0
\end{equation}

Putting it all together:

\begin{equation}
\text{MSE}(h) = \E[(Y - T(X))^2] + \text{CE}(h) + 0
\end{equation}

And substituting \(\E[(Y - T(X))^2]\) with \(\text{Var}[Y] - \text{Var}[T(X)]\), we get:

\begin{equation}
\text{MSE}(h) = \text{Var}[Y] - \text{Var}[T(X)] + \E[(T(X) - h(X))^2]
\end{equation}


\end{answer}