\begin{answer}

Given 
\begin{equation}
    J_\lambda(\beta)=\frac{1}{2}\|X\beta-\vec{y}\|_2^2+\frac{\lambda}{2}\|\beta\|_2^2    
\end{equation}

then
\begin{equation}
    \nabla J_\lambda(\beta) =  X^\top X \beta -  X^\top y + \lambda \beta
\end{equation}

let $\nabla J_\lambda(\beta) = 0$, we get 

\begin{equation}
     X^\top X \beta + \lambda \beta = X^\top y = (X^\top X + \lambda I_{d \times d}) \beta
\end{equation}

then 
\begin{equation}
    \hat{\beta}_\lambda=(X^\top X+\lambda I_{d\times d})^{-1}X^\top \vec{y}
\end{equation}
\end{answer}
